sciostar/case-studies/webserver/Execute.fst
@@ -1,6 +1,7 @@
 module Execute
 
 open FStar.All
+open GuardedDMFree
 open Compiler.Model1
 open Utils
 
@@ -8,13 +9,13 @@ let the_p #a : hist_post #event a = fun lt r -> True
 
 exception Something_went_really_bad
 
-let rec skip_partial_calls (tree: mio mymst int { forall h. dm_mio_theta tree the_p h }) : ML int =
+let rec skip_partial_calls (tree: mio mymst int { forall h. dm_gmio_theta tree the_p h }) : ML int =
   match tree with
   | Return y -> y
-  | PartialCall pre k -> begin
+  | Call (CmdL (GCmd pre)) k -> begin
     (** The intuition here is that the pre-condition is true,
     thus, all asserts are true **)
-   assert (dm_mio_theta tree the_p []);
+   assert (dm_gmio_theta tree the_p []);
    assert pre;
    skip_partial_calls (k ())
   end
@@ -23,12 +24,12 @@ let rec skip_partial_calls (tree: mio mymst int { forall h. dm_mio_theta tree th
   does not exist **)
   | _ -> raise Something_went_really_bad
 
-let cast_mio (wp : hist 'a) (t : dm_mio mymst 'a wp) : (x : mio mymst 'a { dm_mio_theta x ⊑ wp}) =
+let cast_mio (wp : hist 'a) (t : mio_dm mymst 'a wp) : (x : mio mymst 'a { dm_gmio_theta x ⊑ wp}) =
   t
 
 let skip_partial_calls' (dm_tree:dm_gmio int mymst AllOps trivial_hist) : ML int =
-  let dm_tree' : dm_mio mymst int trivial_hist = dm_tree in
-  let dm_tree2 : (x : mio mymst int { dm_mio_theta x ⊑ trivial_hist }) = cast_mio trivial_hist dm_tree' in
+  let dm_tree' : mio_dm mymst int trivial_hist = dm_tree in
+  let dm_tree2 : (x : mio mymst int { dm_gmio_theta x ⊑ trivial_hist }) = cast_mio trivial_hist dm_tree' in
   skip_partial_calls dm_tree2
 
 let execute (w:unit -> MIO int AllOps mymst (fun _ -> True) (fun _ _ _ -> True)) : ML int =
