lib/DMFree.fst
@@ -1,0 +1,135 @@
+module DMFree
+
+open FStar.Classical.Sugar
+open FStar.List.Tot.Base
+open FStar.Tactics
+
+open Free
+include Hist
+
+(** cmd_wp maps each command to a hist-based WP over events.
+    - cmd: command type (parameterizes the free monad)
+    - event: event type (parameterizes the hist monad) *)
+let cmd_wp (cmd:Type -> Type) (event:Type) = #r:Type -> cmd r -> hist #event r
+
+let cmd_wp_sum
+  #cmd1 #cmd2
+  (#event:Type)
+  (cwp1:cmd_wp cmd1 event)
+  (cwp2:cmd_wp cmd2 event)
+  : cmd_wp (cmd_sum cmd1 cmd2) event =
+  fun op ->
+    match op with
+    | CmdL op1 -> cwp1 op1
+    | CmdR op2 -> cwp2 op2
+
+(** Inspired from Kenji Maillard's thesis (2.4.5)
+    NB: the separate val is needed for extraction: without it, the
+    refinements of dm/gdm (where theta appears applied to the two extra
+    hist arguments) trip the substitution bug of FStarLang/FStar#490. **)
+val theta : #a:Type u#a -> #cmd:(Type u#0 -> Type u#e) -> #event:Type -> cwp:cmd_wp cmd event -> m:free cmd a -> hist #event a
+let rec theta #a #cmd #event cwp m =
+  match m with
+  | Return x -> hist_return x
+  | Call op k ->
+      hist_bind (cwp op) (fun ri -> theta cwp (k ri))
+
+let lemma_theta_is_monad_morphism_ret #cmd (#event:Type) (cwp:cmd_wp cmd event) (v:'a) :
+  Lemma (theta cwp (free_return #cmd v) == hist_return v) by (compute ()) = ()
+
+let another_lemma (wp1:hist 'a) (wp2:'a -> hist 'b) (wp3:'a -> hist 'b) p h :
+  Lemma
+    (requires ((forall x. (wp3 x) ⊑ (wp2 x)) /\ hist_bind wp1 wp2 p h))
+    (ensures (hist_bind wp1 wp3 p h)) = ()
+
+let another_lemma' (wp1:hist 'a) (wp2:'a -> hist 'b) (wp3:'a -> hist 'b) :
+  Lemma
+    (requires ((forall x. (wp3 x) ⊑ (wp2 x))))
+    (ensures (hist_bind wp1 wp3 ⊑ hist_bind wp1 wp2)) = ()
+
+private let hist_ord wp1 wp2 = wp2 ⊑ wp1
+
+let rec lemma_theta_is_lax_morphism_bind #a #b #cmd (#event:Type) (cwp:cmd_wp cmd event) (m:free cmd a) (f:a -> free cmd b) :
+  Lemma
+    (theta cwp (free_bind m f) ⊑ hist_bind (theta cwp m) (fun x -> theta cwp (f x))) =
+  match m with
+  | Return x ->
+    calc (hist_ord) {
+      hist_bind (theta cwp m) (fun x -> theta cwp (f x));
+      == {
+        assert (hist_bind (theta cwp (Return x)) (fun x -> theta cwp (f x))
+          == hist_bind (theta cwp m) (fun x -> theta cwp (f x))) by (rewrite_eqs_from_context ())
+      }
+      hist_bind (theta cwp (Return x)) (fun x -> theta cwp (f x));
+      == { _ by (compute ()) } // unfold theta
+      hist_bind (hist_return x) (fun x -> theta cwp (f x));
+      `hist_ord` {} (** here there is an eta that forces us to use `hist_ord` **)
+      theta cwp (f x);
+      == {} // unfold free_bind
+      theta cwp (free_bind (Return x) f);
+      == {}
+      theta cwp (free_bind m f);
+    }
+  | Call op k ->
+    calc (hist_ord) {
+      hist_bind (theta cwp m) (fun x -> theta cwp (f x));
+      == {
+        assert (hist_bind (theta cwp (Call op k)) (fun x -> theta cwp (f x))
+           == hist_bind (theta cwp m) (fun x -> theta cwp (f x))) by (rewrite_eqs_from_context ())
+      }
+      hist_bind (theta cwp (Call op k)) (fun x -> theta cwp (f x));
+      == { _ by (compute ()) } // unfold theta
+      hist_bind (hist_bind (cwp op) (fun ri -> theta cwp (k ri))) (fun x -> theta cwp (f x));
+      `hist_equiv` { lemma_hist_bind_associativity (cwp op) (fun ri -> theta cwp (k ri)) (fun x -> theta cwp (f x)) }
+      hist_bind (cwp op) (fun ri -> hist_bind (theta cwp (k ri)) (fun x -> theta cwp (f x)));
+      `hist_ord` {
+        let rhs1 = fun ri -> hist_bind (theta cwp (k ri)) (fun x -> theta cwp (f x)) in
+        let rhs2 = fun ri -> theta cwp (free_bind (k ri) f) in
+        introduce forall ri. (rhs1 ri) `hist_ord` (rhs2 ri) with begin
+          lemma_theta_is_lax_morphism_bind cwp (k ri) f
+        end;
+        another_lemma' (cwp op) rhs1 rhs2;
+        assert (hist_bind (cwp op) rhs1 `hist_ord` hist_bind (cwp op) rhs2) by (assumption ())
+      }
+      hist_bind (cwp op) (fun ri -> theta cwp (free_bind (k ri) f));
+      == { _ by (compute ()) } // unfold theta
+      theta cwp (Call op (fun ri -> free_bind (k ri) f));
+      `hist_ord` { _ by (compute ()) } // unfold free_bind
+      theta cwp (free_bind (Call op k) f);
+      == {}
+      theta cwp (free_bind m f);
+    }
+
+// The Dijkstra Monad
+type dm (cmd:Type0 -> Type) (event:Type) (cwp:cmd_wp cmd event) (a:Type) (wp:hist #event a) =
+  (m:(free cmd a){theta cwp m ⊑ wp})
+
+let dm_return #cmd (#event:Type) (cwp:cmd_wp cmd event) #a (x : a) : dm cmd event cwp a (hist_return #a #event x) =
+  free_return x
+
+let dm_cmd #cmd (#event:Type) (cwp:cmd_wp cmd event) #r (op:cmd r) :
+  dm cmd event cwp r (hist_bind (cwp op) (fun ri -> hist_return ri)) =
+  Call op Return
+
+#push-options "--z3rlimit 40"
+let dm_bind
+  #cmd (#event:Type) (cwp:cmd_wp cmd event)
+  #a #b
+  (wp_v : hist #event a)
+  (wp_f: a -> hist #event b)
+  (v : dm cmd event cwp a wp_v)
+  (f : (x:a -> dm cmd event cwp b (wp_f x))) :
+  Tot (dm cmd event cwp b (hist_bind wp_v wp_f)) =
+  lemma_theta_is_lax_morphism_bind cwp v f;
+  free_bind v f
+#pop-options
+
+let dm_subcomp #cmd (#event:Type) (cwp:cmd_wp cmd event) #a (wp1 wp2: hist #event a) (f : dm cmd event cwp a wp1) :
+  Pure (dm cmd event cwp a wp2)
+    (requires wp1 ⊑ wp2)
+    (ensures fun _ -> True) =
+  f
+
+let dm_if_then_else #cmd (#event:Type) (cwp:cmd_wp cmd event) #a
+  (wp1 wp2: hist #event a) (f : dm cmd event cwp a wp1) (g : dm cmd event cwp a wp2) (b : bool) : Type =
+  dm cmd event cwp a (hist_if_then_else wp1 wp2 b)
