lib/Free.fst
@@ -1,0 +1,49 @@
+module Free
+
+(** Sum of two command types.
+    Commands are indexed types (Type0 -> Type) parameterizing the free monad. *)
+noeq
+type cmd_sum (cmd1 cmd2 : Type -> Type) : Type -> Type =
+| CmdL : #r:Type -> cmd1 r -> cmd_sum cmd1 cmd2 r
+| CmdR : #r:Type -> cmd2 r -> cmd_sum cmd1 cmd2 r
+
+(** Sum of two event types.
+    Events are plain types parameterizing the hist monad. *)
+noeq
+type event_sum (ev1 ev2 : Type) =
+| EvL : ev1 -> event_sum ev1 ev2
+| EvR : ev2 -> event_sum ev1 ev2
+
+noeq
+type free (cmd : Type u#i -> Type u#e) (a:Type u#a) : Type u#(max (1 + i) (max a e)) =
+| Call : #r:Type u#i -> cmd r -> cont:(r -> free cmd a) -> free cmd a
+| Return : a -> free cmd a
+
+val free_return : #cmd:(Type u#i -> Type u#e) -> #a:Type u#a -> x:a -> free cmd a
+let free_return #cmd #a (x:a) : free cmd a =
+  Return x
+
+val free_bind : #cmd:(Type u#i -> Type u#e) -> #a:Type u#a -> #b:Type u#b -> l:free cmd a -> k:(a -> free cmd b) -> free cmd b
+let rec free_bind
+  #cmd #a #b
+  (l : free cmd a)
+  (k : a -> free cmd b) :
+  free cmd b =
+  match l with
+  | Return x -> k x
+  | Call op fnc ->
+      Call op (fun i ->
+        free_bind (fnc i) k)
+
+val free_map : #cmd:(Type u#i -> Type u#e) -> #a:Type u#a -> #b:Type u#b -> l:free cmd a -> k:(a -> b) -> Tot (free cmd b)
+let free_map
+  #cmd #a #b
+  (l : free cmd a)
+  (k : a -> b) :
+  Tot (free cmd b) =
+  free_bind l (fun x -> free_return (k x))
+
+let free_codomain_ordering
+  #cmd #a
+  (x:(free cmd a){Call? x}) :
+  Lemma (forall r. Call?.cont x r << x) = ()
